shift-reset/core/val.v
@@ -1,0 +1,6 @@
+From shift_reset.core Require Import syntax tag.
+
+Definition VFun' (t : term1) (env : env) : val := VFun (C1 env t).
+Definition VFix' (t : term2) (env : env) : val := VFix (C2 env t).
+Definition VExn' (tag : tag) (v : val) : val := VExn (Exn tag v).
+Definition VEff' (tag : tag) (v : val) : val := VEff (Eff tag v).
